src/Examples/StatDb/Refinement.v
@@ -1,0 +1,62 @@
+From iris.algebra Require Import auth gmap.
+Require Export CSL.Refinement.
+Require Import StatDb.Impl StatDb.WeakestPre.
+Set Default Proof Using "Type".
+
+
+
+Section refinement_triples.
+  Context `{!varG Σ, !lockG Σ, !@cfgG (DB.Op) (DB.l) Σ}.
+  Context (ρ : thread_pool DB.Op * DB.l.(State)).
+
+  Import Var.
+
+  Definition DBLockInv :=
+    (∃ l, source_state l ∗ Sum ↦ (fold_right plus O l) ∗ Count ↦ (length l))%I.
+
+  Definition DBInv := (source_ctx ρ ∗ ∃ N γ, is_lock N γ DBLockInv)%I.
+
+  (* TODO: write smart tactics for applying the wp_primitives *)
+  Lemma add_refinement {T} j (K: unit → proc DB.Op T) n:
+    {{{ j ⤇ Bind (Call (DB.Add n)) K ∗ DBInv }}} add n {{{ RET tt; j ⤇ Bind (Ret tt) K }}}.
+  Proof.
+    iIntros (Φ) "(Hj&#Hsource_inv&Hinv) HΦ".
+    iDestruct "Hinv" as (N γ) "#Hinv".
+    wp_bind. iApply (wp_lock with "[$]").
+    iIntros "!> (Hlocked&HDB)".
+    iDestruct "HDB" as (l) "(Hsource&Hsum&Hcount)".
+    wp_bind. iApply (wp_read with "Hsum"). iIntros "!> Hsum".
+    wp_bind. iApply (wp_write with "[$]"). iIntros "!> Hsum".
+    wp_bind. iApply (wp_read with "Hcount"). iIntros "!> Hcount".
+    wp_bind. iApply (wp_write with "[$]"). iIntros "!> Hcount".
+    iMod (ghost_step_lifting_bind with "Hj Hsource_inv Hsource") as "(Hj&Hsource&_)".
+    { do 2 eexists; split; last by eauto. econstructor. }
+    { set_solver+. }
+    iAssert DBLockInv with "[-HΦ Hlocked Hj]" as "HDB".
+    { iExists _; iFrame. }
+    iApply (wp_unlock with "[-HΦ Hj]"); iFrame.
+    { iFrame "Hinv"; eauto. }
+    iIntros "!> _". by iApply "HΦ".
+  Qed.
+
+  Lemma avg_refinement {T} j (K: nat → proc DB.Op T):
+    {{{ j ⤇ Bind (Call (DB.Avg)) K ∗ DBInv }}} avg {{{ n, RET n; j ⤇ Bind (Ret n) K }}}.
+  Proof.
+    iIntros (Φ) "(Hj&#Hsource_inv&Hinv) HΦ".
+    iDestruct "Hinv" as (N γ) "#Hinv".
+    wp_bind. iApply (wp_lock with "[$]").
+    iIntros "!> (Hlocked&HDB)".
+    iDestruct "HDB" as (l) "(Hsource&Hsum&Hcount)".
+    wp_bind. iApply (wp_read with "Hsum"). iIntros "!> Hsum".
+    wp_bind. iApply (wp_read with "Hcount"). iIntros "!> Hcount".
+    iMod (ghost_step_lifting_bind with "Hj Hsource_inv Hsource") as "(Hj&Hsource&_)".
+    { do 2 eexists; split; last by eauto. econstructor. }
+    { set_solver+. }
+    iAssert DBLockInv with "[-HΦ Hlocked Hj]" as "HDB".
+    { iExists _; iFrame. }
+    wp_bind. iApply (wp_unlock with "[-HΦ Hj]"); iFrame.
+    { iFrame "Hinv"; eauto. }
+    iIntros "!> _".
+    wp_ret. by iApply "HΦ".
+  Qed.
+End refinement_triples.
